unique_ids2.thy
@@ -1,0 +1,168 @@
+theory unique_ids2
+  imports unique_ids
+    invariant_simps 
+    unique_ids
+    single_invocation_correctness2
+    "Case_Labeling.Case_Labeling"
+    execution_invariants2
+    execution_invariants_s
+    execution_invariants_unused
+    impl_language
+    topological_sort
+begin
+
+
+definition 
+  "new_unique_not_in_invocationOp iop uidv \<equiv>
+\<forall>i op. iop i \<triangleq> op \<longrightarrow> to_nat uidv \<notin> uniqueIds op "
+
+
+definition 
+  "new_unique_not_in_calls iop uidv \<equiv>
+\<forall>i op r. iop i \<triangleq> Call op r \<longrightarrow> to_nat uidv \<notin> uniqueIds op "
+
+definition 
+  "new_unique_not_in_calls_result iop uidv \<equiv>
+\<forall>i op r. iop i \<triangleq> Call op r \<longrightarrow> to_nat uidv \<notin> uniqueIds r "
+
+definition
+"new_unique_not_in_invocationRes ires uidv \<equiv> 
+\<forall>i r. ires i \<triangleq> r \<longrightarrow> to_nat uidv \<notin> uniqueIds r "
+
+
+(* TODO hmm, I have the feeling that I already did something similar ... *)
+lemma growth_still_hidden:
+  assumes g: "state_monotonicGrowth i S S'"
+    and prog_wf: "program_wellFormed (prog S)"
+    and a1: "new_unique_not_in_invocationOp (invocationOp S) uidv"
+    and a2: "new_unique_not_in_calls (calls S) uidv"
+    and a3: "new_unique_not_in_calls_result (calls S) uidv"
+    and a4: "new_unique_not_in_invocationRes (invocationRes S) uidv"
+    and a5: "to_nat uidv \<notin> knownIds S"
+    and a6: "generatedIds S (to_nat uidv) \<triangleq> i"
+shows "new_unique_not_in_invocationOp (invocationOp S') uidv
+\<and> new_unique_not_in_calls (calls S') uidv
+\<and> new_unique_not_in_calls_result (calls S') uidv
+\<and> new_unique_not_in_invocationRes (invocationRes S') uidv
+\<and> to_nat uidv \<notin> knownIds S'"
+proof -
+  from g obtain tr
+    where wf: "state_wellFormed S"
+    and steps: "S ~~ tr \<leadsto>* S'"
+    and no_i: "\<forall>x\<in>set tr. case x of (i', a) \<Rightarrow> i' \<noteq> i"
+    and no_fail: "\<forall>i. (i, AFail) \<notin> set tr"
+    by (auto simp add: state_monotonicGrowth_def)
+
+
+  from steps no_i wf no_fail prog_wf a1 a2 a3 a4 a5 a6
+  show ?thesis
+  proof (induct rule: steps.induct)
+    case (steps_refl S)
+    then show ?case
+      by auto
+  next
+    case (steps_step S1 tr S2 a S3)
+
+
+    have "new_unique_not_in_invocationOp (invocationOp S2) uidv \<and>
+        new_unique_not_in_calls (calls S2) uidv \<and>
+        new_unique_not_in_calls_result (calls S2) uidv \<and>
+        new_unique_not_in_invocationRes (invocationRes S2) uidv \<and> to_nat uidv \<notin> knownIds S2"
+      by (rule steps_step, insert `\<forall>i. (i, AFail) \<notin> set (tr @ [a])`,auto simp add: steps_step)
+
+    hence i1: "new_unique_not_in_invocationOp (invocationOp S2) uidv "
+      and i2: "new_unique_not_in_calls (calls S2) uidv "
+      and i3: "new_unique_not_in_calls_result (calls S2) uidv"
+      and i4: "new_unique_not_in_invocationRes (invocationRes S2) uidv"
+      and i5: "to_nat uidv \<notin> knownIds S2"
+      by (auto simp add: steps_step)
+
+    note invs = i1 i2 i3 i4 i5
+   
+
+    from `S2 ~~ a \<leadsto> S3`
+    show ?case
+    proof (induct rule: step.cases)
+      case (local S i ls f ls')
+      then show ?case
+        using invs by (auto simp add: )
+    next
+      case (newId S i ls f ls' uid uidv ls'')
+      then show ?case 
+        using invs by (auto simp add: )
+    next
+      case (beginAtomic S i ls f ls' t vis snapshot)
+      then show ?case using invs by (auto simp add: )
+    next
+      case (endAtomic S i ls f ls' t)
+      then show ?case using invs by (auto simp add: )
+    next
+      case (dbop S i ls f Op ls' t c res vis)
+      from dbop 
+      show ?case using invs 
+      proof (auto simp add: )
+
+        show "new_unique_not_in_calls (\<lambda>a. if a = c then Some (Call Op res) else calls S a) uidv"
+          if c0: "S2 = S"
+            and c1: "a = (i, ADbOp c Op res)"
+            and c2: "S3 = S \<lparr>localState := localState S(i \<mapsto> ls' res), calls := calls S(c \<mapsto> Call Op res), callOrigin := callOrigin S(c \<mapsto> t), visibleCalls := visibleCalls S(i \<mapsto> insert c vis), happensBefore := happensBefore S \<union> vis \<times> {c}\<rparr>"
+            and c3: "localState S i \<triangleq> ls"
+            and c4: "currentProc S i \<triangleq> f"
+            and c5: "f ls = DbOperation Op ls'"
+            and c6: "currentTransaction S i \<triangleq> t"
+            and c7: "calls S c = None"
+            and c8: "querySpec (prog S) Op (getContextH (calls S) (happensBefore S) (Some vis)) res"
+            and c9: "visibleCalls S i \<triangleq> vis"
+            and c10: "new_unique_not_in_invocationOp (invocationOp S) uidv"
+            and c11: "new_unique_not_in_calls (calls S) uidv"
+            and c12: "new_unique_not_in_calls_result (calls S) uidv"
+            and c13: "new_unique_not_in_invocationRes (invocationRes S) uidv"
+            and c14: "to_nat uidv \<notin> knownIds S"
+          sorry
+
+        show "new_unique_not_in_calls_result (\<lambda>a. if a = c then Some (Call Op res) else calls S a) uidv"
+          if c0: "S2 = S"
+            and c1: "a = (i, ADbOp c Op res)"
+            and c2: "S3 = S \<lparr>localState := localState S(i \<mapsto> ls' res), calls := calls S(c \<mapsto> Call Op res), callOrigin := callOrigin S(c \<mapsto> t), visibleCalls := visibleCalls S(i \<mapsto> insert c vis), happensBefore := happensBefore S \<union> vis \<times> {c}\<rparr>"
+            and c3: "localState S i \<triangleq> ls"
+            and c4: "currentProc S i \<triangleq> f"
+            and c5: "f ls = DbOperation Op ls'"
+            and c6: "currentTransaction S i \<triangleq> t"
+            and c7: "calls S c = None"
+            and c8: "querySpec (prog S) Op (getContextH (calls S) (happensBefore S) (Some vis)) res"
+            and c9: "visibleCalls S i \<triangleq> vis"
+            and c10: "new_unique_not_in_invocationOp (invocationOp S) uidv"
+            and c11: "new_unique_not_in_calls (calls S) uidv"
+            and c12: "new_unique_not_in_calls_result (calls S) uidv"
+            and c13: "new_unique_not_in_invocationRes (invocationRes S) uidv"
+            and c14: "to_nat uidv \<notin> knownIds S"
+          sorry
+      qed
+
+
+
+
+
+    next
+      case (invocation S i proc initialState impl)
+      then show ?case using invs apply (auto simp add: )
+        by (auto simp add: new_unique_not_in_invocationOp_def)
+    next
+      case (return S i ls f res)
+      then show ?case using invs apply (auto simp add: )
+         apply (auto simp add: new_unique_not_in_invocationRes_def)
+        sorry
+
+    next
+      case (fail S i ls)
+      then show ?case using invs by (auto simp add: )
+    next
+      case (invCheck S res i)
+      then show ?case using invs by (auto simp add: )
+    qed
+  qed
+qed
+
+
+
+end
